verification, session13
all problems done & solved, just for practising

dafny/session-13/adts-1-all-solved.dfy
@@ -140,7 +140,7 @@ predicate isSkew (t: Skew)
 {
    match t
       case Empty       => true
-      case Node(l,x,r) => isSkew(l) && isSkew(r) &&  heap(l, x, r) 
+      case Node(l,x,r) => isSkew(l) && isSkew(r) && heap(l, x, r) 
 }				
 
 // This is the heap property at the root level
@@ -355,16 +355,168 @@ ensures inorder(mirror(t)) == rev(inorder(t))
 //    and prove the following lemma:
 
 function preorder<T> (t: Tree<T>): seq<T>
+{
+   match t
+      case Empty        => []
+      case Node(l,x,r)  =>
+         [x] + preorder(l) + preorder(r)
+}
 
 function postorder<T> (t: Tree<T>): seq<T>
+{
+   match t
+      case Empty        => []
+      case Node(l,x,r)  =>
+         postorder(l) + postorder(r) + [x]
+}
+
+lemma revLemma3<T>(s1:seq<T>, s2:seq<T>, s3:seq<T>)
+ensures rev(s1+s2+s3) == rev(s3) + rev(s2) + rev(s1)
+{
+   calc == {
+      rev(s1 + s2 + s3);
+      { revLemma2(s3, s1 + s2); }
+      rev(s3) + rev(s1 + s2);
+      { revLemma2(s2, s1); }
+      rev(s3) + rev(s2) + rev(s1);
+   }
+}
+
+lemma revSingle<T> (s1:seq<T>)
+requires |s1| == 1
+ensures rev(s1) == s1
+{}
+
 
 lemma reversePreorder<T> (t: Tree<T>)
 ensures rev(preorder(t)) == postorder(mirror(t))
+{
+   match t
+      case Empty        => {}
+      case Node(l,x,r)  =>
+         {
+            calc == {
+               rev(preorder(t));
+               { assert preorder(t) == [x] + preorder(l) + preorder(r); }
+               rev([x] + preorder(l) + preorder(r));
+               { revLemma3([x], preorder(l), preorder(r)); }
+               rev(preorder(r)) + rev(preorder(l)) + rev([x]);
+               { revSingle([x]); }
+               rev(preorder(r)) + rev(preorder(l)) + [x];
+            }
+         }
+}
 
 // 6. You are given the function flatten and then should program the function merge
 //     which merges two sorted sequences and veryfy both merge and flatten
 
+lemma sortedSeqHead(x:int, s:seq<int>)
+requires sortedSeq(s)
+requires forall e | e in multiset(s) :: x <= e
+ensures sortedSeq([x] + s)
+{
+   if |s| == 0 {
+
+   } else {
+      assert s[0] in multiset(s);
+   }
+}
+
+lemma multisetSeqSum<T> (s1:seq<T>, s2:seq<T>)
+ensures multiset(s1 + s2) == multiset(s1) + multiset(s2)
+{}
+
+lemma multisetSeqSumSingle<T> (s:seq<T>)
+requires |s| > 0
+ensures multiset(s) == multiset{s[0]} + multiset(s[1..])
+{
+   assert s == [s[0]] + s[1..];
+}
+
+lemma multisetIdemp<T> (s1:seq<T>, s2:seq<T>)
+ensures multiset(s1) + multiset(s2) == multiset(s2) + multiset(s1)
+{}
+
+lemma seqSum<T> (s:seq<T>)
+requires |s| > 0
+ensures [s[0]] + s[1..] == s
+{}
+
+function insertSortedSeq(x:int, s:seq<int>) : (res:seq<int>)
+requires sortedSeq(s)
+ensures multiset(res) == multiset(s) + multiset{x}
+ensures sortedSeq(res)
+{
+   if |s| == 0 then
+      [x]
+   else
+      if x <= s[0] then
+         sortedSeqHead(x, s);
+         [x] + s
+      else
+         assert x > s[0];
+         sortedSeqHead(s[0], insertSortedSeq(x, s[1..]));
+         assert multiset(insertSortedSeq(x, s[1..])) == multiset(s[1..]) + multiset{x};
+         multisetSeqSum([s[0]], insertSortedSeq(x, s[1..]));
+         assert multiset([s[0]] + insertSortedSeq(x, s[1..])) == multiset([s[0]]) + multiset(insertSortedSeq(x, s[1..]));
+         assert multiset(insertSortedSeq(x, s[1..])) == multiset{x} + multiset(s[1..]);
+         assert multiset([s[0]] + insertSortedSeq(x, s[1..])) == multiset{x} + multiset([s[0]]) + multiset(s[1..]);
+         seqSum(s);
+         assert multiset([s[0]]) + multiset(s[1..]) == multiset(s);
+         assert multiset([s[0]] + insertSortedSeq(x, s[1..])) == multiset(s) + multiset{x};
+         [s[0]] + insertSortedSeq(x, s[1..])
+}
+
+lemma insertHeadLess (x:int, s:seq<int>)
+requires sortedSeq(s)
+requires |s| > 0
+requires x <= s[0]
+ensures sortedSeq([x] + s)
+{}
+
 function merge(s1: seq<int>, s2: seq<int>): (res:seq<int>)
+requires sortedSeq(s1) && sortedSeq(s2)
+ensures multiset(res) == multiset(s1) + multiset(s2)
+ensures sortedSeq(res)
+decreases s2
+{
+   if |s1| == 0 then
+      s2
+   else
+      if |s2| == 0 then
+         s1
+      else
+         var x := s1[0];
+         var y := s2[0];
+         if x < y then
+            var auxSeq := insertSortedSeq(y, s1[1..]);
+            sortedSeqHead(x, auxSeq);
+            // assert sortedSeq([x] + auxSeq);
+            // assert multiset(merge([x] + auxSeq, s2[1..])) == multiset([x] + auxSeq) + multiset(s2[1..]);
+            multisetSeqSum([x], auxSeq);
+            // assert multiset([x] + auxSeq) + multiset(s2[1..]) == multiset{x} + multiset(s1[1..]) + multiset{y} + multiset(s2[1..]);
+            multisetSeqSumSingle(s1);
+            // assert x == s1[0];
+            // assert multiset(s1) == multiset{x} + multiset(s1[1..]);
+            multisetSeqSumSingle(s2);
+            // assert y == s2[0];
+            // assert multiset(s2) == multiset{y} + multiset(s2[1..]);
+            // assert multiset{x} + multiset(s1[1..]) + multiset{y} + multiset(s2[1..]) == multiset(s1) + multiset(s2);
+            // assert multiset([x] + auxSeq) + multiset(s2[1..]) == multiset(s1) + multiset(s2);
+            // assert multiset(merge([x] + auxSeq, s2[1..])) == multiset(s1) + multiset(s2);
+            merge([x] + auxSeq, s2[1..])
+         else
+            insertHeadLess(y, s1);
+            // assert multiset(merge([y] + s1, s2[1..])) == multiset([y] + s1) + multiset(s2[1..]);
+            multisetSeqSum([y], s1);
+            // assert multiset([y] + s1) == multiset([y]) + multiset(s1);
+            // assert multiset(merge([y] + s1, s2[1..])) == multiset([y]) + multiset(s1) + multiset(s2[1..]);
+            multisetIdemp([y], s1);
+            // assert multiset(merge([y] + s1, s2[1..])) == multiset(s1) + multiset([y]) + multiset(s2[1..]);
+            multisetSeqSumSingle(s2);
+            // assert multiset(merge([y] + s1, s2[1..])) == multiset(s1) + multiset(s2);
+            merge([y] + s1, s2[1..])
+}
 
 
 function flatten(t:Skew):(res:seq<int>)
@@ -376,5 +528,15 @@ ensures sortedSeq(res)
      case Empty       =>   []
      case Node(l,x,r) =>   var left := flatten(l);
                            var right := flatten(r);
+                           // assert heap(l,x,r);
+                           // assert forall e | e in mset(l) + mset(r) :: x <= e;
+                           // assert mset(l) == multiset(left);
+                           // assert mset(r) == multiset(right);
+                           // assert forall e | e in multiset(left) + multiset(right) :: x <= e;
+                           // assert multiset(merge(left, right)) == multiset(left) + multiset(right);
+                           // assert forall e | e in multiset(merge(left, right)) :: x <= e;
+                           // assert sortedSeq(merge(left,right));
+                           sortedSeqHead(x, merge(left,right));
+                           // assert sortedSeq([x] + merge(left,right));
                            [x] + merge(left,right)
 }
